aarch64 refine: update for explicit fpu changes
Signed-off-by: Corey Lewis <corey.lewis@proofcraft.systems>

proof/refine/AARCH64/ADT_H.thy
@@ -263,15 +263,16 @@ lemma FaultMap_fault_map[simp]:
   done
 
 definition
-  "ArchTcbMap atcb \<equiv>
-    \<lparr> tcb_context =  atcbContext atcb, tcb_vcpu = atcbVCPUPtr atcb \<rparr>"
+  "ArchTcbMap atcb is_cur_fpu_owner \<equiv>
+    \<lparr> tcb_context = atcbContext atcb, tcb_vcpu = atcbVCPUPtr atcb, tcb_cur_fpu = is_cur_fpu_owner \<rparr>"
 
 lemma arch_tcb_relation_imp_ArchTcnMap:
-  "\<lbrakk> arch_tcb_relation atcb atcb'\<rbrakk> \<Longrightarrow> ArchTcbMap atcb' = atcb"
+  "\<lbrakk> arch_tcb_relation atcb atcb'; tcb_cur_fpu atcb = is_cur_fpu_owner\<rbrakk>
+   \<Longrightarrow> ArchTcbMap atcb' is_cur_fpu_owner = atcb"
   by (clarsimp simp: arch_tcb_relation_def ArchTcbMap_def)
 
 definition
-  "TcbMap tcb \<equiv>
+  "TcbMap tcb is_cur_fpu_owner \<equiv>
      \<lparr>tcb_ctable = CapabilityMap (cteCap (tcbCTable tcb)),
       tcb_vtable = CapabilityMap (cteCap (tcbVTable tcb)),
       tcb_reply = CapabilityMap (cteCap (tcbReply tcb)),
@@ -286,7 +287,8 @@ definition
       tcb_priority = tcbPriority tcb,
       tcb_time_slice = tcbTimeSlice tcb,
       tcb_domain = tcbDomain tcb,
-      tcb_arch = ArchTcbMap (tcbArch tcb)\<rparr>"
+      tcb_flags = word_to_tcb_flags (tcbFlags tcb),
+      tcb_arch = ArchTcbMap (tcbArch tcb) is_cur_fpu_owner\<rparr>"
 
 definition
  "absCNode sz h a \<equiv> CNode sz (\<lambda>bl.
@@ -297,15 +299,15 @@ definition
 
 definition absHeap ::
   "(machine_word \<rightharpoonup> vmpage_size) \<Rightarrow> (machine_word \<rightharpoonup> nat) \<Rightarrow> (machine_word \<rightharpoonup> pt_type) \<Rightarrow>
-     (machine_word \<rightharpoonup> Structures_H.kernel_object) \<Rightarrow> Structures_A.kheap" where
-  "absHeap ups cns pt_types h \<equiv> \<lambda>x.
+     (machine_word \<rightharpoonup> Structures_H.kernel_object) \<Rightarrow> machine_word option \<Rightarrow> Structures_A.kheap" where
+  "absHeap ups cns pt_types h cur_fpu_owner \<equiv> \<lambda>x.
      case h x of
        Some (KOEndpoint ep) \<Rightarrow> Some (Endpoint (EndpointMap ep))
      | Some (KONotification ntfn) \<Rightarrow> Some (Notification (AEndpointMap ntfn))
      | Some KOKernelData \<Rightarrow> undefined \<comment> \<open>forbidden by pspace_relation\<close>
      | Some KOUserData \<Rightarrow> map_option (ArchObj \<circ> DataPage False) (ups x)
      | Some KOUserDataDevice \<Rightarrow> map_option (ArchObj \<circ> DataPage True) (ups x)
-     | Some (KOTCB tcb) \<Rightarrow> Some (TCB (TcbMap tcb))
+     | Some (KOTCB tcb) \<Rightarrow> Some (TCB (TcbMap tcb (cur_fpu_owner = Some x)))
      | Some (KOCTE cte) \<Rightarrow> map_option (\<lambda>sz. absCNode sz h x) (cns x)
      | Some (KOArch ako) \<Rightarrow> map_option ArchObj (absHeapArch h pt_types x ako)
      | None \<Rightarrow> None"
@@ -440,10 +442,14 @@ lemma absHeap_correct:
   assumes pspace_aligned:  "pspace_aligned s"
   assumes pspace_distinct: "pspace_distinct s"
   assumes valid_objs:      "valid_objs s"
+  assumes valid_cur_fpu:   "valid_cur_fpu s"
   assumes pspace_relation: "pspace_relation (kheap s) (ksPSpace s')"
   assumes ghost_relation:  "ghost_relation (kheap s) (gsUserPages s') (gsCNodes s')
                                            (gsPTTypes (ksArchState s'))"
-  shows "absHeap (gsUserPages s') (gsCNodes s') (gsPTTypes (ksArchState s')) (ksPSpace s') = kheap s"
+  assumes arch_state_relation: "(arch_state s, ksArchState s') \<in> arch_state_relation"
+  shows
+    "absHeap (gsUserPages s') (gsCNodes s') (gsPTTypes (ksArchState s')) (ksPSpace s') (armKSCurFPUOwner (ksArchState s'))
+     = kheap s"
 proof -
   from ghost_relation
   have gsUserPages:
@@ -585,9 +591,12 @@ proof -
                        split: option.splits)
       using valid_objs[simplified valid_objs_def Ball_def dom_def fun_app_def]
       apply (erule_tac x=y in allE)
+      using arch_state_relation valid_cur_fpu[simplified valid_cur_fpu_def]
+      apply (erule_tac x=y in allE)
       apply (clarsimp simp add: cap_relation_imp_CapabilityMap valid_obj_def
                                 valid_tcb_def ran_tcb_cap_cases valid_cap_def2
-                                arch_tcb_relation_imp_ArchTcnMap)
+                                arch_tcb_relation_imp_ArchTcnMap arch_state_relation_def
+                                is_tcb_cur_fpu_def obj_at_def)
      apply (simp add: absCNode_def cte_map_def)
      apply (erule pspace_dom_relatedE[OF _ pspace_relation])
      apply (case_tac ko, simp_all add: tcb_relation_cut_def other_obj_relation_def
@@ -1571,14 +1580,15 @@ definition
   "absArchState s' \<equiv>
    case s' of
      ARMKernelState asid_tbl kvspace vmid_tab next_vmid global_us_vspace current_vcpu
-                    num_list_regs gs_pt_types \<Rightarrow>
+                    num_list_regs gs_pt_types current_fpu_owner \<Rightarrow>
      \<lparr> arm_asid_table = asid_tbl \<circ> ucast,
        arm_kernel_vspace = kvspace,
        arm_vmid_table = map_option ucast \<circ> vmid_tab,
        arm_next_vmid = next_vmid,
        arm_us_global_vspace = global_us_vspace,
        arm_current_vcpu = current_vcpu,
-       arm_gicvcpu_numlistregs = num_list_regs \<rparr>"
+       arm_gicvcpu_numlistregs = num_list_regs,
+       arm_current_fpu_owner = current_fpu_owner \<rparr>"
 
 lemma absArchState_correct:
   "(s,s') \<in> state_relation \<Longrightarrow> absArchState (ksArchState s') = arch_state s"
@@ -1620,7 +1630,7 @@ lemma absExst_correct:
 
 definition
   "absKState s \<equiv>
-   \<lparr>kheap = absHeap (gsUserPages s) (gsCNodes s) (gsPTTypes (ksArchState s)) (ksPSpace s),
+   \<lparr>kheap = absHeap (gsUserPages s) (gsCNodes s) (gsPTTypes (ksArchState s)) (ksPSpace s) (armKSCurFPUOwner (ksArchState s)),
     cdt = absCDT (cteMap (gsCNodes s)) (ctes_of s),
     is_original_cap = absIsOriginalCap (cteMap (gsCNodes s)) (ksPSpace s),
     cur_thread = ksCurThread s, idle_thread = ksIdleThread s,
